theories/examples.v
@@ -15,7 +15,7 @@ Definition demo0 : expr :=
   (* x uses Alias(None) for i *)
 
   (* retag x with new borrow *)
-  Retag "x" Default #0 ;;
+  Retag "x" Default ;;
   (* stack of i: [Uniq(0); Uniq(?)], not frozen *)
   (* x now uses Uniq(0) for i *)
 
@@ -27,7 +27,7 @@ Definition demo0 : expr :=
   (* stack of y  : [Uniq(y)], not frozen *)
 
   (* retag y with new borrow *)
-  Retag "y" Default #0 ;;
+  Retag "y" Default ;;
   (* stack of i: [Uniq(1); Uniq(0); Uniq(?)], not frozen *)
   (* y now uses Uniq(1) for i *)
 
@@ -67,7 +67,7 @@ Definition demo1 : expr :=
   (* x uses Alias(None) for i *)
 
   (* retag x with new borrow *)
-  Retag "x" Default #☠ ;;
+  Retag "x" Default ;;
   (* stack of i: [Uniq(0); Uniq(?)], not frozen *)
   (* x now uses Uniq(0) for i *)
 
@@ -79,7 +79,7 @@ Definition demo1 : expr :=
   (* stack of y1 : [Uniq(y1)], not frozen *)
 
   (* retag y1 with new borrow *)
-  Retag "y1" Default #☠ ;;
+  Retag "y1" Default ;;
   (* stack of i: [Raw; Uniq(0); Uniq(?)], frozen_since(1) *)
   (* y1 now uses Alias(1) for i *)
 
@@ -98,7 +98,7 @@ Definition demo1 : expr :=
   (* stack of y2 : [Uniq(y2)], not frozen *)
 
   (* retag y2 with new borrow *)
-  Retag "y2" Default #☠ ;;
+  Retag "y2" Default ;;
   (* stack of i: [Raw; Uniq(0); Uniq(?)], frozen_since(1) *)
   (* y2 now uses Alias(2) for i *)
 
@@ -130,7 +130,7 @@ Definition demo2 : expr :=
   (* x uses Alias(None) for the int *)
 
   (* retag x with new borrow *)
-  Retag "x" Default #☠ ;;
+  Retag "x" Default ;;
   (* stack of iint: [Uniq(0); Uniq(?)], not frozen *)
   (* x now uses Uniq(0) for i *)
 
@@ -142,7 +142,7 @@ Definition demo2 : expr :=
   (* stack of y : [Uniq(y)], not frozen *)
 
   (* retag y with new borrow *)
-  Retag "y" Default #☠ ;;
+  Retag "y" Default ;;
   (* stack of i: [Raw; Uniq(0); Uniq(?)], frozen_since(1) *)
   (* y now uses Alias(1) for i *)
 
@@ -156,7 +156,7 @@ Definition demo2 : expr :=
   (* stack of z : [Uniq(z)], not frozen *)
 
   (* retag z with new borrow *)
-  Retag "z" RawRt #☠ ;;
+  Retag "z" RawRt ;;
   (* stack of i: [Raw; Uniq(0); Uniq(?)], frozen_since(1) *)
   (* z now uses Alias(None) for the int *)
 
@@ -191,7 +191,7 @@ Definition demo4 : expr :=
   (* x uses Alias(None) for i *)
 
   (* retag x with new borrow *)
-  Retag "x" Default #☠ ;;
+  Retag "x" Default ;;
   (* stack of int: [Uniq(0); Uniq(?)], not frozen *)
   (* x now uses Uniq(0) for i *)
 
@@ -203,7 +203,7 @@ Definition demo4 : expr :=
   (* stack of y1 : [Uniq(y1)], not frozen *)
 
   (* retag y with new borrow *)
-  Retag "y1" RawRt #☠ ;;
+  Retag "y1" RawRt ;;
   (* stack of i: [Raw; Uniq(0); Uniq(?)], not frozen *)
   (* y1 now uses Alias(None) for i *)
 
@@ -215,7 +215,7 @@ Definition demo4 : expr :=
   (* stack of y2  : [Uniq(y2)], not frozen *)
 
   (* retag y2 with new borrow *)
-  Retag "y2" RawRt #☠ ;;
+  Retag "y2" RawRt ;;
   (* stack of i : [Raw; Uniq(0); Uniq(?)], not frozen *)
   (* y2 now uses Alias(None) for i *)
 
